cv_translator/eval_cake_compile_ag32Lib.sml
@@ -9,10 +9,12 @@ local
   open eval_cake_compileLib;
 
   val ag32_arch_thms =
-    { default_config_def = ag32_configTheory.ag32_backend_config_def
-    , to_livesets_def    = backend_ag32Theory.to_livesets_ag32_def
-    , compile_cake_def   = backend_ag32Theory.compile_cake_ag32_def
-    , cv_export_def      = backend_ag32_cvTheory.cv_ag32_export_def } : arch_thms;
+    { default_config_def  = ag32_configTheory.ag32_backend_config_def
+    , default_config_simp = backend_ag32_cvTheory.set_asm_conf_ag32_backend_config
+    , to_livesets_def     = backend_ag32Theory.to_livesets_ag32_def
+    , compile_cake_def    = backend_ag32Theory.compile_cake_ag32_def
+    , compile_cake_imp    = backend_ag32Theory.compile_cake_ag32_thm
+    , cv_export_def       = backend_ag32_cvTheory.cv_ag32_export_def } : arch_thms;
 
 in
 
