compiler/backend/backendScript.sml
@@ -812,4 +812,50 @@ Definition ffinames_to_string_list_def:
     ffinames_to_string_list rest)
 End
 
+
+Definition inc_set_oracle_def:
+  inc_set_oracle c oracle =
+    c with inc_word_to_word_conf :=
+        (c.inc_word_to_word_conf with col_oracle := oracle)
+End
+
+Definition set_oracle_def:
+  set_oracle c oracle =
+    c with
+    word_to_word_conf := c.word_to_word_conf with col_oracle := oracle
+End
+
+Definition set_asm_conf_def:
+  set_asm_conf c asm_c =
+    c with lab_conf := c.lab_conf with asm_conf := asm_c
+End
+
+Theorem inc_set_oracle_pull:
+  ∀oracle c. inc_config_to_config b (inc_set_oracle c oracle) =
+             set_oracle (inc_config_to_config b c) oracle
+Proof
+  gvs [inc_set_oracle_def,inc_config_to_config_def,set_oracle_def]
+QED
+
+Theorem inc_config_to_config_config_to_inc_config:
+  inc_config_to_config asm_c (config_to_inc_config c) =
+  set_asm_conf c asm_c
+Proof
+  gvs [inc_config_to_config_def,
+       config_to_inc_config_def,
+       lab_to_targetTheory.inc_config_to_config_def,
+       lab_to_targetTheory.config_to_inc_config_def,
+       config_component_equality,
+       lab_to_targetTheory.config_component_equality,
+       set_asm_conf_def]
+QED
+
+Theorem set_asm_conf_id:
+  c.lab_conf.asm_conf = asm_c ⇒
+  set_asm_conf c asm_c = c
+Proof
+  gvs [set_asm_conf_def, fetch "-" "config_component_equality",
+       lab_to_targetTheory.config_component_equality]
+QED
+
 val _ = export_theory();
