cv_translator/backend_arm8_cvScript.sml
@@ -3,6 +3,7 @@
 *)
 open preamble cv_transLib cv_stdTheory backend_cvTheory backend_64_cvTheory;
 open backend_arm8Theory arm8Theory arm8_targetTheory to_data_cvTheory;
+open export_arm8Theory arm8_configTheory;
 
 val _ = new_theory "backend_arm8_cv";
 
@@ -262,6 +263,14 @@ val _ = cv_auto_trans
 
 val _ = cv_trans backend_arm8Theory.to_livesets_arm8_def;
 val _ = cv_trans backend_arm8Theory.compile_cake_arm8_def;
+
+(* lemma used by automation *)
+
+Theorem set_asm_conf_arm8_backend_config:
+  set_asm_conf arm8_backend_config arm8_config = arm8_backend_config
+Proof
+  irule backendTheory.set_asm_conf_id \\ EVAL_TAC
+QED
 
 val _ = Feedback.set_trace "TheoryPP.include_docs" 0;
 val _ = export_theory();
