examples/pseudo_bool/array/compilation/npbc_fullCompileScript.sml
@@ -1,11 +1,11 @@
 (*
   Compiles the PB checker example by evaluation inside the logic of HOL
 *)
-open preamble compilationLib npbc_fullProgTheory
+open preamble npbc_fullProgTheory eval_cake_compile_x64Lib
 
 val _ = new_theory "npbc_fullCompile"
 
-val pb_arrayFull_compiled = save_thm("npbc_full_compiled",
-  compile_x64 "cake_pb" main_prog_def);
+Theorem npbc_full_compiled =
+  eval_cake_compile_x64 "" main_prog_def "cake_pb.S";
 
 val _ = export_theory ();
