examples/pseudo_bool/array/compilation/subgraph_isoCompileScript.sml
@@ -1,11 +1,11 @@
 (*
   Compiles the encoder
 *)
-open preamble compilationLib subgraph_isoProgTheory
+open preamble subgraph_isoProgTheory eval_cake_compile_x64Lib
 
 val _ = new_theory "subgraph_isoCompile"
 
-val subgraph_iso_compiled = save_thm("subgraph_iso_compiled",
-  compile_x64 "cake_pb_iso" main_prog_def);
+Theorem subgraph_iso_compiled =
+  eval_cake_compile_x64 "" main_prog_def "cake_pb_iso.S";
 
 val _ = export_theory ();
