examples/pseudo_bool/array/compilation/wcnfCompileScript.sml
@@ -1,11 +1,11 @@
 (*
   Compiles the WCNF + PB checker
 *)
-open preamble compilationLib wcnfProgTheory
+open preamble wcnfProgTheory eval_cake_compile_x64Lib
 
 val _ = new_theory "wcnfCompile"
 
-val wcnf_compiled = save_thm("wcnf_compiled",
-  compile_x64 "cake_pb_wcnf" main_prog_def);
+Theorem wcnf_compiled =
+  eval_cake_compile_x64 "" main_prog_def "cake_pb_wcnf.S";
 
 val _ = export_theory ();
