examples/pseudo_bool/array/compilation/README.md
@@ -12,10 +12,16 @@ Compiles the MCCIS + PB checker
 [mcisCompileScript.sml](mcisCompileScript.sml):
 Compiles the MCIS + PB checker
 
+[npbc_fullCompileARM8Script.sml](npbc_fullCompileARM8Script.sml):
+Compiles the PB checker example by evaluation inside the logic of HOL
+
 [npbc_fullCompileScript.sml](npbc_fullCompileScript.sml):
 Compiles the PB checker example by evaluation inside the logic of HOL
 
 [proofs](proofs):
+Prove end-to-end correctness theorem for PB checker with arrays
+
+[proofsARM8](proofsARM8):
 Prove end-to-end correctness theorem for PB checker with arrays
 
 [subgraph_isoCompileScript.sml](subgraph_isoCompileScript.sml):
